Added getNAlmostExpired() and getAlmostExpired() with sequence, need to do with array

verification/PacketPile.dfy
@@ -181,4 +181,55 @@ class PacketPile
     {
         c := this.count;
     }
+    
+    function method Count(a: seq<int>, key: int) : nat
+        decreases |a|
+    {   
+        if |a| == 0 then 0 else
+        (if a[0] == key then 1 else 0) + Count(a[1..], key)
+    }
+
+    lemma DistributiveLemma(a: seq<int>, b: seq<int>, key: int)
+        ensures Count(a + b, key) == Count(a, key) + Count(b, key)
+    {
+        if a == [] {
+            assert a + b == b;
+        } else {
+            DistributiveLemma(a[1..], b, key);
+            assert a + b == [a[0]] + (a[1..] + b);
+        }
+    }
+
+    method getNAlmostExpired() returns (n: int)
+        requires Valid(); ensures Valid()
+        ensures n == Count(buf[..], 1)
+    {
+        n := Count(buf[..], 1);
+    }
+
+    // Need to verify with arrays
+    method getAlmostExpired() returns (trash: seq<int>)
+        requires Valid(); ensures Valid()
+        ensures forall i :: 0 <= i < |trash| ==> trash[i] == 1;
+    {
+        var size := getNAlmostExpired();
+        //trash := new int[size];
+        trash := [];
+        var i := 0;
+        var next := 0;
+        while i < count
+        decreases count - i
+        invariant 0 <= i <= count
+        //invariant 1 in buf[..i] <==> next > 0
+        invariant 0 <= next <= i
+        invariant forall j :: 0 <= j < |trash| ==> trash[j] == 1
+        {
+            if buf[i] == 1 {
+                //trash[next] := buf[i];
+                //next := next + 1;
+                trash := trash + [buf[i]];
+            }
+            i := i + 1;
+        }
+    }
 }
